Split compile.v into types, functions and modules

theories/compiler/functions.v
@@ -1,44 +1,42 @@
 From Coq Require Import List.
+Import Coq.Lists.List.ListNotations.
 Require Import Coq.Program.Basics.
 Require Import Coq.Strings.String.
-Import Coq.Lists.List.ListNotations.
 Require Import Coq.NArith.BinNat.
 Require Import Coq.ZArith.BinInt.
 Local Open Scope program_scope.
 
-Require Import mathcomp.ssreflect.seq.
-
-From stdpp Require Import -(notations) list_numbers pretty.
-
-From ExtLib.Structures Require Import Functor Monads Reducible Traversable.
-Import FunctorNotation.
-Import MonadNotation.
-Local Open Scope monad.
 From ExtLib.Data Require Import List.
 From ExtLib.Data.Monads Require Import EitherMonad StateMonad WriterMonad.
+From ExtLib.Structures Require Import Monads Reducible Traversable.
+Import MonadNotation.
+Local Open Scope monad.
+
+From stdpp Require Import -(notations) list_numbers.
 
 From Wasm Require datatypes operations.
 Require Import Wasm.numerics.
 
-From RichWasm Require term.
-From RichWasm Require Import typing.
+From RichWasm Require term typing.
+From RichWasm.compiler Require Import error numerics types.
 Require Import RichWasm.util.dlist.
 Import RichWasm.util.dlist.Notation.
-From RichWasm.compiler Require Import numerics util.
 
-Module R := term.
-Module W := datatypes.
-
-(* Mapping from size variables to indices of locals of type i32 *)
-Definition size_ctx := list W.immediate.
+Module R. Include term <+ typing. End R.
+Module W. Include datatypes <+ operations. End W.
 
 (* locals exclusive to webassembly (compiler-generated temporaries, etc) *)
-Definition wlocal_ctx := list W.value_type.
+Notation wlocal_ctx := (list W.value_type).
 
 Notation instr_list := (dlist W.basic_instruction).
 
 Record wst (A : Type) :=
-  { un_wst : stateT wlocal_ctx (writerT (@DList.Monoid_dlist W.basic_instruction) (sum err)) A }.
+  { un_wst : stateT
+               wlocal_ctx
+               (writerT
+                  (@DList.Monoid_dlist W.basic_instruction)
+                  (sum error))
+               A }.
 
 Arguments Build_wst {A} _.
 Arguments un_wst {A} _.
@@ -49,7 +47,7 @@ Global Instance Monad_wst : Monad wst :=
   { ret := fun _ x => Build_wst (ret x);
     bind := fun _ _ c f => Build_wst (bind (un_wst c) (fun x => un_wst (f x))) }.
 
-Global Instance MonadExc_wst : MonadExc err wst :=
+Global Instance MonadExc_wst : MonadExc error wst :=
   { raise := fun _ e => Build_wst (raise e);
     catch := fun _ body hnd => Build_wst (catch (un_wst body) (fun e => un_wst (hnd e))) }.
 
@@ -66,10 +64,27 @@ Global Instance MonadWriter_wst : MonadWriter (@DList.Monoid_dlist W.basic_instr
       pass ('(a, t, s) <- runStateT (un_wst c) s;;
             ret (a, s, t)))) }.
 
-Definition lift_err {A} (c : err + A) : wst A :=
+Record compiler_mod_ctx :=
+  { mem_gc : W.immediate;
+    mem_lin : W.immediate;
+    free : W.immediate;
+    alloc : W.immediate;
+    registerroot : W.immediate;
+    unregisterroot : W.immediate;
+    duproot : W.immediate;
+    coderef_offset : W.immediate;
+    fn_tab : W.immediate }.
+
+Definition lift_error {A} (c : error + A) : wst A :=
   Build_wst (lift (lift c)).
 
-Definition run_compiler (c : wst unit) (wl : wlocal_ctx) : err + wlocal_ctx * list W.basic_instruction :=
+Definition try_option {A} (e : error) (x : option A) : wst A :=
+  match x with
+  | None => raise e
+  | Some x' => ret x'
+  end.
+
+Definition run_compiler (c : wst unit) (wl : wlocal_ctx) : error + wlocal_ctx * list W.basic_instruction :=
   match runWriterT (runStateT (un_wst c) wl) with
   | inl e => inl e
   | inr x => inr (snd (PPair.pfst x), DList.to_list (PPair.psnd x))
@@ -97,131 +112,8 @@ Definition if_c {A B} (tf : W.function_type) (thn : wst A) (els : wst B) : wst (
   emit (W.BI_if tf (DList.to_list es1) (DList.to_list es2));;
   ret (x1, x2).
 
-Record compiler_mod_ctx := {
-  mem_gc : W.immediate;
-  mem_lin : W.immediate;
-  free : W.immediate;
-  alloc : W.immediate;
-  registerroot : W.immediate;
-  unregisterroot : W.immediate;
-  duproot : W.immediate;
-  coderef_offset : W.immediate;
-  fn_tab : W.immediate;
-}.
-
-Definition compile_int_type (typ : R.IntType) : W.value_type :=
-  match typ with
-  | R.i32 => W.T_i32
-  | R.i64 => W.T_i64
-  end.
-
-Definition compile_float_type (typ : R.FloatType) : W.value_type :=
-  match typ with
-  | R.f32 => W.T_f32
-  | R.f64 => W.T_f64
-  end.
-
-Definition compile_numtyp (typ: R.NumType) : W.value_type :=
-  match typ with
-  | R.Int _ inttyp => compile_int_type inttyp
-  | R.Float floattyp => compile_float_type floattyp
-  end.
-
-Definition compile_kindvar (κ: R.KindVar) : list W.value_type :=
-  match κ with
-  | R.SIZE _ _ => [W.T_i32]
-  | _ => []
-  end.
-
-Definition compile_kindvars (κs: list R.KindVar) : list W.value_type :=
-  flat_map compile_kindvar κs.
-
-Fixpoint compile_typ (typ: R.Typ) : list W.value_type :=
-  match typ with
-  | R.Num ntyp => [compile_numtyp ntyp]
-  | R.TVar _ => [W.T_i32]
-  | R.Unit => []
-  | R.ProdT typs => flatten (map compile_typ typs)
-  | R.CoderefT _ => [W.T_i32]
-  | R.Rec _ typ => compile_typ typ
-  | R.PtrT _ => [W.T_i32]
-  | R.ExLoc q typ => compile_typ typ
-  | R.OwnR _ => []
-  | R.CapT _ _ _ => []
-  | R.RefT _ _ _  => [W.T_i32]
-  end.
-
-Definition compile_arrow_type (typ: R.ArrowType) : W.function_type :=
-  match typ with
-  | R.Arrow tys1 tys2 =>
-    let tys1' := mapT compile_typ tys1 in
-    let tys2' := mapT compile_typ tys2 in
-    W.Tf (flatten tys1') (flatten tys2')
-  end.
-
-Definition compile_fun_type (ft: R.FunType) : W.function_type :=
-  match ft with
-  | R.FunT κs (R.Arrow tys1 tys2) =>
-    let κvs := compile_kindvars κs in
-    let tys1' := flatten (mapT compile_typ tys1) in
-    let tys2' := flatten (mapT compile_typ tys2) in
-    W.Tf (κvs ++ tys1') tys2'
-  end.
-
-Definition words_typ (typ: R.Typ) : nat :=
-  sum_list_with operations.words_t (compile_typ typ).
-
-Definition throw_missing (instr_name : string) : err + W.basic_instruction :=
-  inl (Err ("missing iris-wasm " ++ instr_name ++ " wrap instruction")).
-
-Definition compile_num (num_type : R.NumType) (num : nat) : W.value :=
-  match num_type with
-  | R.Int _ R.i32 =>
-    W.VAL_int32 (Wasm_int.int_of_Z numerics.i32m (Z.of_nat num))
-  | R.Int _ R.i64 =>
-    W.VAL_int64 (Wasm_int.int_of_Z numerics.i64m (Z.of_nat num))
-  (* is the signed converter the right thing to use here? *)
-  | R.Float R.f32 =>
-    W.VAL_float32
-      (Wasm_float.float_convert_si32
-         numerics.f32m (Wasm_int.int_of_Z numerics.i32m (Z.of_nat num)))
-  | R.Float R.f64 =>
-    W.VAL_float64
-      (Wasm_float.float_convert_si64
-         numerics.f64m (Wasm_int.int_of_Z numerics.i64m (Z.of_nat num)))
-  end.
-
-Fixpoint expect_concrete_size (sz: R.Size) : err + nat :=
-  match sz with
-  | R.SizeConst c => inr c
-  | R.SizePlus sz1 sz2 =>
-      c1 <- expect_concrete_size sz1;;
-      c2 <- expect_concrete_size sz2;;
-      inr (c1 + c2)
-  | _ => inl (Err "expected concrete size")
-  end.
-
-Fixpoint struct_field_offset (fields: list (R.Typ * R.Size)) (idx: nat) : err + R.Size :=
-  match idx with
-  | 0 => inr (R.SizeConst 0)
-  | S idx' =>
-      match fields with
-      | (_, sz) :: fields' => R.SizePlus sz <$> struct_field_offset fields' idx'
-      | [] => inl Todo
-      end
-  end.
-
-Definition get_struct_field_types (targs : list R.Typ) (idx : nat) : err + list (R.Typ * R.Size) :=
-  match lookup idx targs with
-  | Some (R.RefT _ _ (R.StructType fields)) => inr fields
-  | _ => inl (Err ("struct instruction expected type-args to be a ref to a struct at index " ++ pretty idx))
-  end.
-
-Definition get_array_elem_type (targs : list R.Typ) (idx : nat) : err + R.Typ :=
-  match lookup idx targs with
-  | Some (R.RefT _ _ (R.ArrayType typ)) => inr typ
-  | _ => inl (Err ("array instruction expected a ref to an array type at index " ++ pretty idx))
-  end.
+(* Mapping from size variables to indices of locals of type i32 *)
+Definition size_ctx := list W.immediate.
 
 Definition if_gc_bit_set {A} {B}
   (tf : W.function_type)
@@ -248,7 +140,7 @@ Fixpoint loads'
   | ty :: tys =>
       emit (W.BI_get_local base_ptr_var);;
       emit (W.BI_load mem ty None 0%N off);;
-      loads' base_ptr_var mem (off + N.of_nat (operations.length_t ty))%N tys
+      loads' base_ptr_var mem (off + N.of_nat (W.length_t ty))%N tys
   end.
 
 Definition loads mem base_ptr_var tys : wst unit :=
@@ -266,7 +158,7 @@ Fixpoint loc_stores'
       emit (W.BI_get_local base_ptr_var);;
       emit (W.BI_get_local val_var);;
       emit (W.BI_store mem ty None 0%N off);;
-      loc_stores' base_ptr_var mem (off + N.of_nat (operations.length_t ty))%N val_var_tys
+      loc_stores' base_ptr_var mem (off + N.of_nat (W.length_t ty))%N val_var_tys
   end.
 
 Definition loc_stores base_ptr_var mem val_var_tys : wst unit :=
@@ -288,36 +180,6 @@ Definition scope_get_set (scope : VarScope) :
   | VSLocal => (W.BI_get_local, W.BI_set_local)
   end.
 
-Inductive LayoutMode :=
-  | LMWords
-  | LMNative.
-
-Definition layout_ty_length (layout : LayoutMode) (ty : R.Typ) :=
-  match layout with
-  | LMWords => words_typ ty
-  | LMNative => length (compile_typ ty)
-  end.
-
-Definition ref_indices (layout : LayoutMode) (ty : R.Typ) : list W.immediate :=
-  let fix go ty i :=
-    match ty with
-    | R.Num _
-    | R.Unit
-    | R.CoderefT _
-    | R.PtrT _
-    | R.OwnR _
-    | R.CapT _ _ _ => []
-    | R.ProdT tys =>
-        snd (foldl (fun '(j, is) ty' => (j + layout_ty_length layout ty', is ++ go ty' j))
-                   (i, [])
-                   tys)
-    | R.Rec _ ty'
-    | R.ExLoc _ ty' => go ty' i
-    | R.TVar _
-    | R.RefT _ _ _ => [i]
-    end in
-  go ty 0.
-
 Definition for_gc_ref_vars (scope : VarScope) (vars : list W.immediate) (m : wst unit) : wst unit :=
   iterM
     (fun var =>
@@ -331,7 +193,7 @@ Section Mod.
 
   (* TODO: should these be combined? *)
   Variable mctx : compiler_mod_ctx.
-  Variable C : Module_Ctx.
+  Variable C : R.Module_Ctx.
 
   Definition tagged_store
     (base_ptr: W.immediate)
@@ -362,9 +224,9 @@ Section Mod.
 
   Section Fun.
 
-    Variable (sz_locs: size_ctx).
-    Variable (F : Function_Ctx).
-    Variable (temps_off : nat).
+    Variable sz_locs: size_ctx.
+    Variable F : R.Function_Ctx.
+    Variable temps_off : nat.
 
     Definition wnext : wst W.immediate :=
       temps <- get;;
@@ -393,14 +255,17 @@ Section Mod.
       forT tys walloc_rvalue;;
       ret i.
 
-    Fixpoint local_layout (L: Local_Ctx) (base: nat) (i: nat) : err + (nat * R.Typ) :=
-      match L, i with
-      | (τ, sz) :: L, 0 => inr (base, τ)
-      | (τ, sz) :: L, S i =>
-          sz_const <- expect_concrete_size sz;;
-          local_layout L (base + sz_const) i
-      | [], _ => inl (Err "local_layout given out of bounds index")
-      end.
+    Definition local_layout (L : R.Local_Ctx) (idx : nat) : error + (nat * R.Typ) :=
+      let fix go L base i :=
+        match L, i with
+        | (τ, sz) :: L, 0 => inr (base, τ)
+        | (τ, sz) :: L, S i =>
+            sz_const <- size_upper_bound F.(R.size) sz;;
+            go L (base + sz_const) i
+        | [], _ => inl (ELocalIndexOutOfBounds idx)
+        end
+      in
+      go L 0 idx.
 
     Definition gc_loads
       (ref_var: W.immediate)
@@ -566,8 +431,7 @@ Section Mod.
     Fixpoint compile_sz (sz : R.Size) : wst unit :=
       match sz with
       | R.SizeVar σ =>
-        local_idx <- lift_err (err_opt (lookup σ sz_locs)
-                                       ("sz " ++ pretty σ ++ " not found in sz_local_map"));;
+        local_idx <- try_option (ESizeIndexOutOfBounds σ) (lookup σ sz_locs);;
         emit (W.BI_get_local local_idx)
       | R.SizePlus sz1 sz2 =>
         compile_sz sz1;;
@@ -600,14 +464,14 @@ Section Mod.
       emit (W.BI_const (W.VAL_int32 (Wasm_int.int_of_Z i32m (Z.of_nat 4))));; (* skip header length word *)
       emit (W.BI_binop W.T_i32 (W.Binop_i W.BOI_add)).
 
-    Fixpoint compile_instr (instr: R.instr TyAnn) : wst unit :=
+    Fixpoint compile_instr (instr: R.instr R.TyAnn) : wst unit :=
       match instr with
       | R.INumConst _ num_type num => emit (W.BI_const (compile_num num_type num))
       | R.IUnit _ => ret tt
-      | R.INum ann ni => lift_err (compile_num_instr ni) >>= emit
+      | R.INum ann ni => emit (compile_num_instr ni)
       | R.IUnreachable (R.Arrow targs trets, _) => emit (W.BI_unreachable)
       | R.INop (R.Arrow targs trets, _) => emit (W.BI_nop)
-      | R.IDrop (R.Arrow targs trets, LSig L _) =>
+      | R.IDrop (R.Arrow targs trets, R.LSig L _) =>
           match targs with
           | [t_drop] =>
               let wasm_typ := compile_typ t_drop in
@@ -617,7 +481,7 @@ Section Mod.
               restore_stack [t_drop] base;;
               forT wasm_typ (const (emit W.BI_drop));;
               ret tt
-          | _ => raise (Err "drop should consume exactly one value")
+          | _ => raise EWrongTypeAnn
           end
       | R.IBlock (R.Arrow targs trets, _) ta _ es =>
           block_c (compile_arrow_type ta) (forT es compile_instr);;
@@ -633,7 +497,7 @@ Section Mod.
       | R.IBrIf (R.Arrow targs trets, _) x => emit (W.BI_br_if x)
       | R.IBrTable (R.Arrow targs trets, _) x x0 => emit (W.BI_br_table x x0)
       | R.IRet (R.Arrow targs trets, _) =>
-          let ret_ty' := ssrfun.Option.default [] F.(rettyp) in
+          let ret_ty' := ssrfun.Option.default [] F.(R.rettyp) in
           let rdropped := take (length targs - length ret_ty') targs in
           let wdropped := flat_map compile_typ rdropped in
           idx_ret <- save_stack ret_ty';;
@@ -642,27 +506,27 @@ Section Mod.
           for_gc_ref_vars VSLocal ref_vars (emit (W.BI_call mctx.(unregisterroot)));;
           restore_stack ret_ty' idx_ret;;
           emit W.BI_return
-      | R.IGetLocal (R.Arrow targs trets, LSig L _) idx _ =>
-          '(base, τ) <- lift_err (local_layout L 0 idx);;
+      | R.IGetLocal (R.Arrow targs trets, R.LSig L _) idx _ =>
+          '(base, τ) <- lift_error (local_layout L idx);;
           local_gets τ base;;
           'i <- save_stack [τ];;
           let ref_vars := map (Nat.add i) (ref_indices LMNative τ) in
           for_gc_ref_vars VSLocal ref_vars (emit (W.BI_call mctx.(duproot)));;
           restore_stack [τ] i
-      | R.ISetLocal (R.Arrow targs trets, LSig L _) idx =>
-          '(base, τ) <- lift_err (local_layout L 0 idx);;
+      | R.ISetLocal (R.Arrow targs trets, R.LSig L _) idx =>
+          '(base, τ) <- lift_error (local_layout L idx);;
           let ref_vars := map (Nat.add base) (ref_indices LMWords τ) in
           for_gc_ref_vars VSLocal ref_vars (emit (W.BI_call mctx.(unregisterroot)));;
           local_sets τ base
       | R.IGetGlobal _ i =>
-          '(i', ty) <- lift_err (err_opt (global_layout C.(global) i) "invalid global index");;
+          '(i', ty) <- try_option (EGlobalIndexOutOfBounds i) (global_layout C.(R.global) i);;
           forT (imap (fun j _ => i' + j) (compile_typ ty)) (emit ∘ W.BI_get_global);;
           j <- save_stack [ty];;
           let ref_vars := map (Nat.add j) (ref_indices LMNative ty) in
           for_gc_ref_vars VSLocal ref_vars (emit (W.BI_call mctx.(duproot)));;
           restore_stack [ty] i
       | R.ISetGlobal _ i =>
-          '(i', ty) <- lift_err (err_opt (global_layout C.(global) i) "invalid global index");;
+          '(i', ty) <- try_option (EGlobalIndexOutOfBounds i) (global_layout C.(R.global) i);;
           let ref_vars := map (Nat.add i') (ref_indices LMNative ty) in
           for_gc_ref_vars VSGlobal ref_vars (emit (W.BI_call mctx.(unregisterroot)));;
           forT (imap (fun j _ => i' + j) (compile_typ ty)) (emit ∘ W.BI_set_global);;
@@ -692,15 +556,15 @@ Section Mod.
           (* load args into locals *)
           (* do an IStructSet on each arg *)
           (* return the base pointer *)
-          raise Todo
+          raise ETodo
       | R.IStructFree (R.Arrow targs trets, _) =>
           (* TODO: unregisterroot fields that may be refs to GC if this struct is MM *)
           emit (W.BI_call mctx.(free))
       | R.IStructGet (R.Arrow from to, _) n =>
           base_ref <- walloc W.T_i32;;
-          fields <- lift_err (get_struct_field_types from 0);;
-          field_typ <- lift_err (err_opt (list_lookup 0 to) "struct.get: cannot find output val type");;
-          offset_sz <- lift_err (struct_field_offset fields n);;
+          fields <- lift_error (get_struct_field_types from 0);;
+          field_typ <- try_option EWrongTypeAnn (lookup 0 to);;
+          offset_sz <- lift_error (struct_field_offset fields n);;
           emit (W.BI_tee_local base_ref);;
           tagged_load base_ref (compile_sz offset_sz) field_typ;;
           stk <- save_stack [field_typ];;
@@ -712,10 +576,10 @@ Section Mod.
           restore_stack [field_typ] stk
       | R.IStructSet (R.Arrow from to, _) n =>
           base_ref <- walloc W.T_i32;;
-          fields <- lift_err (get_struct_field_types from 1);;
-          field_typ <- lift_err (err_opt (list_lookup 0 to) "struct.set: cannot find output val type");;
-          val_typ <- lift_err (err_opt (list_lookup 0 from) "struct.set: cannot find input val type");;
-          offset_sz <- lift_err (struct_field_offset fields n);;
+          fields <- lift_error (get_struct_field_types from 1);;
+          field_typ <- try_option EWrongTypeAnn (lookup 0 to);;
+          val_typ <- try_option EWrongTypeAnn (lookup 0 from);;
+          offset_sz <- lift_error (struct_field_offset fields n);;
 
           emit (W.BI_tee_local base_ref);;
           if_gc_bit_set (W.Tf [] [])
@@ -740,27 +604,15 @@ Section Mod.
           tagged_store' (compile_sz offset_sz) val_typ
       | R.IStructSwap (R.Arrow from to, _) n =>
           (* TODO: registerroot if GC struct *)
-          fields <- lift_err (get_struct_field_types from 1);;
-          field_typ <- lift_err (err_opt (list_lookup 0 from) "struct.swap: cannot find input val type");;
-          let field_shape := compile_typ field_typ in
-          offset_sz <- lift_err (struct_field_offset fields n);;
-          offset_e <- compile_sz offset_sz;;
-          raise Todo
-    (*
-          mret $ [layout.Swap] ++                (* [ptr; val] → [val; ptr]*)
-                 offset_e ++                     (* [] → [offset] *)
-                 [layout.SwapOffset field_shape; (* [ptr; offset; val__new] → [ptr; offset; val__old] *)
-                  layout.Swap;                   (* [offset; val] → [val; offset] *)
-                  layout.Drop]                   (* [offset] → [] *)
-    *)
+          raise ETodo
       | R.IVariantMalloc (R.Arrow from to, _) sz tys q =>
           (* TODO: registerroot on the new address;
                    unregisterroot if payload is GC ref being put into GC variant *)
-          typ <- lift_err (err_opt (list_lookup 0 from) "variant.malloc: cannot find val type");;
+          typ <- try_option EWrongTypeAnn (lookup 0 from);;
           let shape := compile_typ typ in
           (* memory layout is [ind, τ*] so we just add prepend *)
           (*let full_shape := LS_tuple [LS_int32; shape] in*)
-          raise Todo (*
+          raise ETodo (*
           mret $ [
             layout.Val $ LV_int32 (shape_size_words full_shape);
             layout.Malloc;                                       (* [i32] → [ptr] *)
@@ -773,15 +625,15 @@ Section Mod.
         *)
       | R.IVariantCase ann q th ta tl es =>
           (* TODO: duproot if unrestricted *)
-          raise Todo
+          raise ETodo
           (* [val__init; len] → [ptr] *)
           (* [τ      ; i32] → [i32] *)
       | R.IArrayMalloc (R.Arrow from to, _) q =>
           (* TODO: unregisterroot the initial value if GC array;
                    duproot a bunch of times if MM array *)
-          arr_init_typ <- lift_err (err_opt (list_lookup 1 from) "array.malloc: cannot find val type");;
+          arr_init_typ <- try_option EWrongTypeAnn (list_lookup 1 from);;
           let shape := compile_typ arr_init_typ in
-          raise Todo
+          raise ETodo
                  (*
           mret [
             layout.Dup;             (* [len] → [len; len] *)
@@ -802,7 +654,7 @@ Section Mod.
             | 1   | 1 * 2  |
             ...
             | i   | i * 2  | *)
-          elem_typ <- lift_err (get_array_elem_type from 1);;
+          elem_typ <- lift_error (get_array_elem_type from 1);;
           let elem_shape := compile_typ elem_typ in
           idx_local <- walloc W.T_i32;;
           base_local <- walloc W.T_i32;;
@@ -836,7 +688,7 @@ Section Mod.
              | 1   | 2 * 2       |
              ...
              | i   | (i + 1) * 2 | *)
-          elem_typ <- lift_err (get_array_elem_type from 2);;
+          elem_typ <- lift_error (get_array_elem_type from 2);;
           let elem_shape := compile_typ elem_typ in
           idx_local <- walloc W.T_i32;;
           base_local <- walloc W.T_i32;;
@@ -853,13 +705,13 @@ Section Mod.
           ret tt
       | R.IArrayFree ann =>
           (* TODO: unregisterroot a bunch of times, since this is an MM array *)
-          raise Todo (*mret $ [wasm.BI_call Σ.(me_free)]*)
+          raise ETodo (*mret $ [wasm.BI_call Σ.(me_free)]*)
       | R.IExistPack (R.Arrow targs trets, _) t th q =>
           (* TODO: unregisterroot if GC package *)
-          raise Todo
+          raise ETodo
       | R.IExistUnpack (R.Arrow targs trets, _) q th ta tl es =>
           (* TODO: registerroot if GC package *)
-          raise Todo
+          raise ETodo
       | R.IRefSplit _
       | R.IRefJoin _
       | R.IRecFold _ _
@@ -873,91 +725,9 @@ Section Mod.
       | R.IQualify _ _ => ret tt
       end.
 
-      Definition compile_instrs : list (R.instr TyAnn) -> wst unit :=
+      Definition compile_instrs : list (R.instr R.TyAnn) -> wst unit :=
         iterM compile_instr.
 
   End Fun.
 
 End Mod.
-
-Definition compile_fun_type_idx (fun_type : R.FunType) : W.typeidx.
-Admitted.
-
-Definition funcidx_table_write : W.immediate := 0.
-
-Definition typeidx_start : W.immediate := 0.
-
-Definition typeidx_table_write : W.immediate := 1.
-
-Definition globidx_table_next : W.immediate := 0.
-
-Definition globidx_table_offset : W.immediate := 1.
-
-Definition compile_table_elem (start : W.immediate) (i funcidx : nat) : W.expr :=
-  [ W.BI_get_local start;
-    W.BI_const (W.VAL_int32 (Wasm_int.int_of_Z i32m (Z.of_nat i)));
-    W.BI_binop W.T_i32 (W.Binop_i W.BOI_add);
-    W.BI_const (W.VAL_int32 (Wasm_int.int_of_Z i32m (Z.of_nat funcidx)));
-    W.BI_call funcidx_table_write ].
-
-Definition compile_start (table : R.Table) : W.module_func :=
-  {| W.modfunc_type := W.Mk_typeidx typeidx_start;
-     W.modfunc_locals := [];
-     W.modfunc_body :=
-       [ (* Remember the starting index of our section in the table. *)
-         W.BI_get_global globidx_table_next;
-         W.BI_set_global globidx_table_offset;
-         (* Increment the index for the next module to use the table. *)
-         W.BI_get_global globidx_table_offset;
-         W.BI_const (W.VAL_int32 (Wasm_int.int_of_Z i32m (Z.of_nat (length table))));
-         W.BI_binop W.T_i32 (W.Binop_i W.BOI_add);
-         W.BI_set_global globidx_table_next ] ++
-       flatten (imap (compile_table_elem 0) table) |}.
-
-Fixpoint compile_module (module : R.module TyAnn) : err + W.module :=
-  let '(funcs, globs, table) := module return err + W.module in
-  let mctx := {|
-    mem_gc := 0;
-    mem_lin := 1;
-    free := 1;
-    alloc := 2;
-    registerroot := 3;
-    unregisterroot := 4;
-    duproot := 5;
-    coderef_offset := 0;
-    fn_tab := 0;
-  |} in
-  inr {|
-    W.mod_types := []; (* TODO *)
-    W.mod_funcs := []; (* TODO *)
-    W.mod_tables := []; (* TODO *)
-    W.mod_mems := []; (* TODO *)
-    W.mod_globals := (* TODO *)
-      [ W.Build_module_glob
-          (W.Build_global_type W.MUT_mut W.T_i32)
-          [ W.BI_const (W.VAL_int32 (Wasm_int.int_of_Z i32m 0)) ] ];
-    W.mod_elem := []; (* TODO *)
-    W.mod_data := []; (* TODO *)
-    W.mod_start := Some (W.Build_module_start (W.Mk_funcidx 0)); (* TODO *)
-    W.mod_imports := (* TODO *)
-      [ W.Build_module_import
-          (String.list_byte_of_string "RichWasm")
-          (String.list_byte_of_string "modify_table")
-          (W.ID_func typeidx_table_write) ];
-    W.mod_exports := [] (* TODO *)
-  |}
-
-(* TODO: modfunc_type expects a typeidx while rwasm does this inline *)
-with compile_func (func : R.Func TyAnn) : option W.module_func :=
-  match func with
-  | R.Fun exports fun_type sizes intrs =>
-    Some {|
-      W.modfunc_type := compile_fun_type_idx fun_type;
-      W.modfunc_locals := []; (* TODO *)
-      W.modfunc_body := []; (* TODO *)
-    |}
-  end
-
-with compile_glob (glob : R.Glob TyAnn) : err + W.module_glob
-with compile_table (table : R.Table) : err + W.module_table.
-Admitted.
