theories/compiler/error.v
@@ -1,0 +1,6 @@
+Inductive error :=
+  | EWrongTypeAnn
+  | EGlobalIndexOutOfBounds (index : nat)
+  | ELocalIndexOutOfBounds (index : nat)
+  | ESizeIndexOutOfBounds (index : nat)
+  | ETodo.
