theories/compiler/modules.v
@@ -1,0 +1,101 @@
+From Coq Require Import List.
+Require Import Coq.Program.Basics.
+Require Import Coq.Strings.String.
+Import Coq.Lists.List.ListNotations.
+Require Import Coq.NArith.BinNat.
+Require Import Coq.ZArith.BinInt.
+Local Open Scope program_scope.
+
+Require Import mathcomp.ssreflect.seq.
+
+From stdpp Require Import -(notations) list_numbers pretty.
+
+From ExtLib.Structures Require Import Functor Monads Reducible Traversable.
+Import FunctorNotation.
+Import MonadNotation.
+Local Open Scope monad.
+From ExtLib.Data Require Import List.
+From ExtLib.Data.Monads Require Import EitherMonad StateMonad WriterMonad.
+
+From Wasm Require datatypes operations.
+Require Import Wasm.numerics.
+
+From RichWasm Require term.
+From RichWasm Require Import typing.
+Require Import RichWasm.util.dlist.
+Import RichWasm.util.dlist.Notation.
+From RichWasm.compiler Require Import error functions numerics types.
+
+Module R := term.
+Module W := datatypes.
+
+Definition compile_fun_type_idx (fun_type : R.FunType) : W.typeidx.
+Admitted.
+
+Definition funcidx_table_write : W.immediate := 0.
+
+Definition typeidx_start : W.immediate := 0.
+
+Definition typeidx_table_write : W.immediate := 1.
+
+Definition globidx_table_next : W.immediate := 0.
+
+Definition globidx_table_offset : W.immediate := 1.
+
+Definition compile_table_elem (start : W.immediate) (i funcidx : nat) : W.expr :=
+  [ W.BI_get_local start;
+    W.BI_const (W.VAL_int32 (Wasm_int.int_of_Z i32m (Z.of_nat i)));
+    W.BI_binop W.T_i32 (W.Binop_i W.BOI_add);
+    W.BI_const (W.VAL_int32 (Wasm_int.int_of_Z i32m (Z.of_nat funcidx)));
+    W.BI_call funcidx_table_write ].
+
+Definition compile_start (table : R.Table) : W.module_func :=
+  {| W.modfunc_type := W.Mk_typeidx typeidx_start;
+     W.modfunc_locals := [];
+     W.modfunc_body :=
+       [ (* Remember the starting index of our section in the table. *)
+         W.BI_get_global globidx_table_next;
+         W.BI_set_global globidx_table_offset;
+         (* Increment the index for the next module to use the table. *)
+         W.BI_get_global globidx_table_offset;
+         W.BI_const (W.VAL_int32 (Wasm_int.int_of_Z i32m (Z.of_nat (length table))));
+         W.BI_binop W.T_i32 (W.Binop_i W.BOI_add);
+         W.BI_set_global globidx_table_next ] ++
+       flatten (imap (compile_table_elem 0) table) |}.
+
+Fixpoint compile_module (module : R.module TyAnn) : error + W.module :=
+  let '(funcs, globs, table) := module in
+  inr {|
+    W.mod_types := []; (* TODO *)
+    W.mod_funcs := []; (* TODO *)
+    W.mod_tables := []; (* TODO *)
+    W.mod_mems := []; (* TODO *)
+    W.mod_globals := (* TODO *)
+      [ W.Build_module_glob
+          (W.Build_global_type W.MUT_mut W.T_i32)
+          [ W.BI_const (W.VAL_int32 (Wasm_int.int_of_Z i32m 0)) ] ];
+    W.mod_elem := []; (* TODO *)
+    W.mod_data := []; (* TODO *)
+    W.mod_start := Some (W.Build_module_start (W.Mk_funcidx 0)); (* TODO *)
+    W.mod_imports := (* TODO *)
+      [ W.Build_module_import
+          (String.list_byte_of_string "RichWasm")
+          (String.list_byte_of_string "modify_table")
+          (W.ID_func typeidx_table_write) ];
+    W.mod_exports := [] (* TODO *)
+  |}
+
+(* TODO: modfunc_type expects a typeidx while rwasm does this inline *)
+with compile_func (func : R.Func TyAnn) : option W.module_func :=
+  match func with
+  | R.Fun exports fun_type sizes intrs =>
+    Some {|
+      W.modfunc_type := compile_fun_type_idx fun_type;
+      W.modfunc_locals := []; (* TODO *)
+      W.modfunc_body := []; (* TODO *)
+    |}
+  end
+
+with compile_glob (glob : R.Glob TyAnn) : error + W.module_glob
+with compile_table (table : R.Table) : error + W.module_table.
+Admitted.
