theories/compiler/types.v
@@ -1,0 +1,143 @@
+From Coq Require Import List.
+Import ListNotations.
+
+Require Import mathcomp.ssreflect.seq.
+
+From stdpp Require Import -(notations) list_numbers.
+
+From ExtLib.Data Require Import List.
+From ExtLib.Structures Require Import Functor Monads Traversable.
+Import FunctorNotation MonadNotation.
+Local Open Scope monad.
+
+From Wasm Require datatypes operations.
+
+From RichWasm Require term.
+From RichWasm.compiler Require Import error.
+
+Module R := RichWasm.term.
+Module W := Wasm.datatypes.
+
+Inductive LayoutMode :=
+  | LMWords
+  | LMNative.
+
+Definition compile_int_type (typ : R.IntType) : W.value_type :=
+  match typ with
+  | R.i32 => W.T_i32
+  | R.i64 => W.T_i64
+  end.
+
+Definition compile_float_type (typ : R.FloatType) : W.value_type :=
+  match typ with
+  | R.f32 => W.T_f32
+  | R.f64 => W.T_f64
+  end.
+
+Definition compile_numtyp (typ: R.NumType) : W.value_type :=
+  match typ with
+  | R.Int _ inttyp => compile_int_type inttyp
+  | R.Float floattyp => compile_float_type floattyp
+  end.
+
+Definition compile_kindvar (κ: R.KindVar) : list W.value_type :=
+  match κ with
+  | R.SIZE _ _ => [W.T_i32]
+  | _ => []
+  end.
+
+Definition compile_kindvars (κs: list R.KindVar) : list W.value_type :=
+  flat_map compile_kindvar κs.
+
+Fixpoint compile_typ (typ: R.Typ) : list W.value_type :=
+  match typ with
+  | R.Num ntyp => [compile_numtyp ntyp]
+  | R.TVar _ => [W.T_i32]
+  | R.Unit => []
+  | R.ProdT typs => flatten (map compile_typ typs)
+  | R.CoderefT _ => [W.T_i32]
+  | R.Rec _ typ => compile_typ typ
+  | R.PtrT _ => [W.T_i32]
+  | R.ExLoc q typ => compile_typ typ
+  | R.OwnR _ => []
+  | R.CapT _ _ _ => []
+  | R.RefT _ _ _  => [W.T_i32]
+  end.
+
+Definition compile_arrow_type (typ: R.ArrowType) : W.function_type :=
+  match typ with
+  | R.Arrow tys1 tys2 =>
+    let tys1' := mapT compile_typ tys1 in
+    let tys2' := mapT compile_typ tys2 in
+    W.Tf (flatten tys1') (flatten tys2')
+  end.
+
+Definition compile_fun_type (ft: R.FunType) : W.function_type :=
+  match ft with
+  | R.FunT κs (R.Arrow tys1 tys2) =>
+    let κvs := compile_kindvars κs in
+    let tys1' := flatten (mapT compile_typ tys1) in
+    let tys2' := flatten (mapT compile_typ tys2) in
+    W.Tf (κvs ++ tys1') tys2'
+  end.
+
+Definition words_typ (typ: R.Typ) : nat :=
+  sum_list_with operations.words_t (compile_typ typ).
+
+Definition layout_ty_length (layout : LayoutMode) (ty : R.Typ) :=
+  match layout with
+  | LMWords => words_typ ty
+  | LMNative => length (compile_typ ty)
+  end.
+
+Fixpoint size_upper_bound (ctx : list (list R.Size * list R.Size)) (sz : R.Size) : error + nat :=
+  match sz with
+  | R.SizeConst c => inr c
+  | R.SizePlus sz1 sz2 =>
+      ub1 <- size_upper_bound ctx sz1;;
+      ub2 <- size_upper_bound ctx sz2;;
+      inr (ub1 + ub2)
+  | R.SizeVar _ => inl ETodo
+  end.
+
+Fixpoint struct_field_offset (fields: list (R.Typ * R.Size)) (idx: nat) : error + R.Size :=
+  match idx with
+  | 0 => inr (R.SizeConst 0)
+  | S idx' =>
+      match fields with
+      | (_, sz) :: fields' => R.SizePlus sz <$> struct_field_offset fields' idx'
+      | [] => inl ETodo
+      end
+  end.
+
+Definition get_struct_field_types (targs : list R.Typ) (idx : nat) : error + list (R.Typ * R.Size) :=
+  match lookup idx targs with
+  | Some (R.RefT _ _ (R.StructType fields)) => inr fields
+  | _ => inl EWrongTypeAnn
+  end.
+
+Definition get_array_elem_type (targs : list R.Typ) (idx : nat) : error + R.Typ :=
+  match lookup idx targs with
+  | Some (R.RefT _ _ (R.ArrayType typ)) => inr typ
+  | _ => inl EWrongTypeAnn
+  end.
+
+Definition ref_indices (layout : LayoutMode) (ty : R.Typ) : list W.immediate :=
+  let fix go ty i :=
+    match ty with
+    | R.Num _
+    | R.Unit
+    | R.CoderefT _
+    | R.PtrT _
+    | R.OwnR _
+    | R.CapT _ _ _ => []
+    | R.ProdT tys =>
+        snd (foldl (fun '(j, is) ty' => (j + layout_ty_length layout ty', is ++ go ty' j))
+                   (i, [])
+                   tys)
+    | R.Rec _ ty'
+    | R.ExLoc _ ty' => go ty' i
+    | R.TVar _
+    | R.RefT _ _ _ => [i]
+    end in
+  go ty 0.
